One opaque proof shouldn't be opaque

test-suite/erasure_live_test.v
@@ -1,3 +1,4 @@
+From Coq Require Import Recdef.
 From MetaCoq.Template Require Import Loader.
 From MetaCoq.Erasure Require Import SafeTemplateErasure.
 From Coq Require Import String.
@@ -30,3 +31,381 @@ Quote Recursively Definition singlelim := ((fun (X : Set) (x : X) (e : x = x) =>
                   end)).
 
 Time Eval lazy in test singlelim.
+
+Quote Recursively Definition plusr := (plus 0 1).
+
+Eval lazy in test plusr.
+
+
+(** vector addition **)
+Require Coq.Vectors.Vector.
+Print Fin.t.
+Print Vector.t.
+
+Definition vplus {n:nat} :
+  Vector.t nat n -> Vector.t nat n -> Vector.t nat n := (Vector.map2 plus).
+Definition v01 : Vector.t nat 2 :=
+  (Vector.cons nat 0 1 (Vector.cons nat 1 0 (Vector.nil nat))).
+Definition v23 : Vector.t nat 2 :=
+  (Vector.cons nat 2 1 (Vector.cons nat 3 0 (Vector.nil nat))).
+Definition vplus0123 := (vplus v01 v23).
+Quote Recursively Definition cbv_vplus0123 := (* [program] of Coq's answer *)
+  ltac:(let t:=(eval cbv in (vplus0123)) in exact t).
+Print cbv_vplus0123.
+(* [Term] of Coq's answer *)
+Definition ans_vplus0123 := Eval lazy in test cbv_vplus0123.
+
+(* [program] of the program *)
+Quote Recursively Definition p_vplus0123 := vplus0123.
+Time Eval lazy in test p_vplus0123. (* 5s *)
+(*
+  Time Eval vm_compute in test p_vplus0123. (* 3.54s *)
+Time Eval native_compute in test p_vplus0123. (* 23.54s on first run *)
+
+Time Eval native_compute in test p_vplus0123. (* 2.8s on second run *)
+*)
+
+(** Ackermann **)
+Fixpoint ack (n m:nat) {struct n} : nat :=
+  match n with
+    | 0 => S m
+    | S p => let fix ackn (m:nat) {struct m} :=
+                 match m with
+                   | 0 => ack p 1
+                   | S q => ack p (ackn q)
+                 end
+             in ackn m
+  end.
+Definition ack35 := (ack 3 5).
+Quote Recursively Definition cbv_ack35 :=
+  ltac:(let t:=(eval cbv in ack35) in exact t).
+Print cbv_ack35.
+Eval lazy in test cbv_ack35.
+
+(* [program] of the program *)
+Quote Recursively Definition p_ack35 := ack35.
+Print p_ack35.
+Time Eval lazy in test p_ack35. (* 0.041 *)
+
+(** mutual recursion **)
+Inductive tree (A:Set) : Set :=
+  node : A -> forest A -> tree A
+with forest (A:Set) : Set :=
+     | leaf : A -> forest A
+     | fcons : tree A -> forest A -> forest A.
+Arguments leaf {A}.
+Arguments fcons {A}.
+Arguments node {A}.
+Definition sf: forest bool := (fcons (node true (leaf false)) (leaf true)).
+Quote Recursively Definition p_sf := sf.
+Eval cbv in test p_sf.
+
+Fixpoint tree_size (t:tree bool) : nat :=
+  match t with
+    | node a f => S (forest_size f)
+  end
+with forest_size (f:forest bool) : nat :=
+       match f with
+         | leaf b => 1
+         | fcons t f1 => (tree_size t + forest_size f1)
+       end.
+
+Definition arden: forest bool :=
+  fcons (node true (fcons (node true (leaf false)) (leaf true)))
+        (fcons (node true (fcons (node true (leaf false)) (leaf true)))
+               (leaf false)).
+Quote Recursively Definition p_arden := arden.
+Definition arden_size := (forest_size arden).
+Quote Recursively Definition cbv_arden_size :=
+  ltac:(let t:=(eval cbv in arden_size) in exact t).
+Definition ans_arden_size :=
+  Eval cbv in test cbv_arden_size.
+(* [program] of the program *)
+Quote Recursively Definition p_arden_size := arden_size.
+Print p_arden_size.
+Definition P_arden_size := Eval cbv in test p_arden_size.
+Print P_arden_size.
+
+(** SASL tautology function: variable arity **)
+Require Import Bool.
+Fixpoint tautArg (n:nat) : Type :=
+  match n with
+    | 0 => bool
+    | S n => bool -> tautArg n
+  end.
+Fixpoint taut (n:nat) : tautArg n -> bool :=
+  match n with
+    | 0 => (fun x => x)
+    | S n => fun x => taut n (x true) && taut n (x false)
+  end.
+(* Pierce *)
+Definition pierce := taut 2 (fun x y => implb (implb (implb x y) x) x).
+Quote Recursively Definition cbv_pierce :=
+  ltac:(let t:=(eval cbv in pierce) in exact t).
+Print cbv_pierce.
+Definition ans_pierce :=
+  Eval cbv in (test cbv_pierce).
+Print ans_pierce.
+(* [program] of the program *)
+Quote Recursively Definition p_pierce := pierce.
+Print p_pierce.
+Definition P_pierce := Eval cbv in test p_pierce.
+Print P_pierce.
+(* Goal
+  let env := (env P_pierce) in
+  let main := (main P_pierce) in
+  wcbvEval (env) 200 (main) = Ret ans_pierce.
+  vm_compute. reflexivity.
+Qed.
+ *)(* S combinator *)
+Definition Scomb := taut 3
+         (fun x y z => implb (implb x (implb y z))
+                             (implb (implb x y) (implb x z))).
+Quote Recursively Definition cbv_Scomb :=
+  ltac:(let t:=(eval cbv in Scomb) in exact t).
+Print cbv_Scomb.
+Definition ans_Scomb :=
+  Eval cbv in (test cbv_Scomb).
+Print ans_Scomb.
+(* [program] of the program *)
+Quote Recursively Definition p_Scomb := Scomb.
+Print p_Scomb.
+Definition P_Scomb := Eval cbv in (test p_Scomb).
+Print P_Scomb.
+(* Goal
+  let env := (env P_Scomb) in
+  let main := (main P_Scomb) in
+  wcbvEval (env) 200 (main) = Ret ans_pierce.
+  vm_compute. reflexivity.
+Qed.
+ *)
+(** Fibonacci **)
+Fixpoint slowFib (n:nat) : nat :=
+  match n with
+    | 0 => 0
+    | S m => match m with
+               | 0 => 1
+               | S p => slowFib p + slowFib m
+             end
+  end.
+Definition slowFib3 := (slowFib 3).
+Quote Recursively Definition cbv_slowFib3 :=
+  ltac:(let t:=(eval cbv in slowFib3) in exact t).
+Definition ans_slowFib3 :=
+  Eval cbv in (test cbv_slowFib3).
+(* [program] of the program *)
+Quote Recursively Definition p_slowFib3 := slowFib3.
+Definition P_slowFib3 := Eval cbv in (test p_slowFib3).
+(* Goal
+  let env := (env P_slowFib3) in
+  let main := (main P_slowFib3) in
+  wcbvEval (env) 30 (main) = Ret ans_slowFib3.
+  vm_compute. reflexivity.
+Qed.
+ *)
+(* fast Fib *)
+Fixpoint fibrec (n:nat) (fs:nat * nat) {struct n} : nat :=
+  match n with
+    | 0 => fst fs
+    | (S n) => fibrec n (pair ((fst fs) + (snd fs)) (fst fs))
+  end.
+Definition fib : nat -> nat := fun n => fibrec n (pair 0 1).
+Definition fib9 := fib 9.
+Quote Recursively Definition cbv_fib9 :=
+  ltac:(let t:=(eval cbv in fib9) in exact t).
+Definition ans_fib9 :=
+  Eval cbv in (test cbv_fib9).
+(* [program] of the program *)
+Quote Recursively Definition p_fib9 := fib9.
+Definition P_fib9 := Eval cbv in (test p_fib9).
+(* 
+Goal
+  let env := (env P_fib9) in
+  let main := (main P_fib9) in
+  wcbvEval (env) 1000 (main) = Ret ans_fib9.
+  vm_compute. reflexivity.
+Qed.
+ *)
+
+Module HetList.
+(** Heterogenous datatypes, a la Matthes **)
+Inductive PList : Set->Type:=  (* powerlists *)
+| zero : forall A:Set, A -> PList A
+| succ : forall A:Set, PList (A * A)%type -> PList A.
+Arguments zero {A}.
+Arguments succ {A}.
+Definition myPList : PList nat :=
+  succ (succ (succ (zero (((1,2),(3,4)),((5,6),(7,8)))))).
+Unset Asymmetric Patterns.
+Fixpoint unzip {A:Set} (l:list (A*A)) {struct l} : list A :=
+  match l return list A with
+    | nil => nil
+    | cons (a1,a2) l' => cons a1 (cons a2 (unzip l'))
+  end.
+Fixpoint PListToList {A:Set} (l:PList A) {struct l} : list A :=
+  match l in PList A return list A with
+    | zero a => cons a (nil )
+    | succ l' => unzip (PListToList l')
+  end.
+
+Eval compute in PListToList myPList.
+
+Fixpoint gen_sumPList {A:Set} (l:PList A) {struct l} : (A->nat)->nat :=
+  match l in PList A return (A->nat)->nat with
+    | zero a => fun f => f a
+    | succ l' =>
+      fun f => gen_sumPList l' (fun a => let (a1,a2) := a in f a1 + f a2)
+  end.
+Definition sumPList l := gen_sumPList l (fun x => x).
+Definition sumPL_myPL := (sumPList myPList).
+Quote Recursively Definition cbv_sumPL_myPL :=
+  ltac:(let t:=(eval cbv in sumPL_myPL) in exact t).
+Definition ans_sumPL_myPL :=
+  Eval cbv in (test cbv_sumPL_myPL).
+(* [program] of the program *)
+Quote Recursively Definition p_sumPL_myPL := sumPL_myPL.
+Definition P_sumPL_myPL := Eval cbv in (test p_sumPL_myPL).
+(* Goal
+  let env := (env P_sumPL_myPL) in
+  let main := (main P_sumPL_myPL) in
+  wcbvEval (env) 1000 (main) = Ret ans_sumPL_myPL.
+  vm_compute. reflexivity.
+Qed.
+ *)
+
+Set Implicit Arguments.
+Section List.
+Variables X Y : Type.
+Variable f : X -> Y -> Y.
+Fixpoint fold (y : Y) (xs : list X) : Y :=
+  match xs with
+    | nil => y
+    | cons x xr => fold (f x y) xr
+  end.
+End List.
+Inductive Tree := T : list Tree -> Tree.
+Fixpoint size (t : Tree) : nat :=
+  match t with
+    | T ts => S (fold (fun t a => size t + a) 0 ts)
+  end.
+  Definition unit {A} (a : A) : list A := cons a nil.
+  Definition myTree :=
+  (T (cons (T (unit (T nil))) (cons (T (unit (T nil))) nil))).
+
+Eval cbv in size myTree.
+Definition size_myTree := size myTree.
+Quote Recursively Definition cbv_size_myTree :=
+  ltac:(let t:=(eval cbv in size_myTree) in exact t).
+Definition ans_size_myTree :=
+  Eval cbv in (test cbv_size_myTree).
+(* [program] of the program *)
+Quote Recursively Definition p_size_myTree := size_myTree.
+Definition P_size_myTree := Eval cbv in (test p_size_myTree).
+(* Goal
+  let env := (env P_size_myTree) in
+  let main := (main P_size_myTree) in
+  wcbvEval (env) 100 (main) = Ret ans_size_myTree.
+  vm_compute. reflexivity.
+Qed.
+ *)
+End HetList.
+
+Require Import Coq.Arith.Compare_dec.
+Require Import Coq.Arith.PeanoNat.
+Require Import Coq.Arith.Peano_dec.
+Require Import Arith.
+Program Fixpoint provedCopy (n:nat) {wf lt n} : nat :=
+  match n with 0 => 0 | S k => S (provedCopy k) end.
+  Next Obligation.  apply lt_wf. Defined.
+Print Assumptions provedCopy.
+Quote Recursively Definition pCopy := provedCopy. (* program *)
+
+Definition x := 3.
+Definition provedCopyx := provedCopy x.
+Compute provedCopyx.  (** evals correctly in Coq **)
+Quote Recursively Definition cbv_provedCopyx :=
+  ltac:(let t:=(eval cbv in provedCopyx) in exact t).
+Definition ans_provedCopyx :=
+  Eval cbv in (test cbv_provedCopyx).
+Quote Recursively Definition p_provedCopyx := provedCopyx. (* program *)
+(* We don't run those every time as they are really expensive *)
+(* Time Definition P_provedCopyx := Eval lazy in (test p_provedCopyx).
+ *)(* 2 min purely inside Coq *)
+(* Time Definition P_provedCopyxvm := Eval vm_compute in (test p_provedCopyx).
+ *)
+From MetaCoq.Erasure Require Import Loader.
+MetaCoq Erase provedCopyx.
+(* 2m purely in the bytecode VM *)
+(* Time Definition P_provedCopyxvm := Eval native_compute in (test p_provedCopyx).
+(* Anomaly: compilation failure *)
+ *)
+
+(* Goal
+  let env := (env P_provedCopyx) in
+  let main := (main P_provedCopyx) in
+  wcbvEval (env) 100 (main) = Ret ans_provedCopyx.
+  vm_compute. reflexivity.
+Qed.
+ *)
+
+
+ (* debug code in case something is stuck *)
+ (*
+ From MetaCoq.SafeChecker Require Import PCUICSafeChecker.
+
+Definition fold_matchdecl {A B} (e : EnvCheck A) (b : A -> B) (c : PCUICAst.global_env_ext -> env_error -> B) :=
+    match e with
+    |CorrectDecl a => b a
+    |EnvError g a => c g a
+    end.
+
+Ltac fold_matchdecls' := repeat
+    match goal with
+    |- context C [?x] => 
+    match x with 
+    | match ?l with CorrectDecl a => @?b a | EnvError g a' => @?c g a' end =>
+    change x with (fold_matchdecl l b c)
+    end
+    end.
+        
+
+    Set Printing Depth 20.
+
+    
+Ltac eval_first :=
+match goal with
+|- context C [fold_matchdecl ?l ?p ?g] =>
+  match l with
+  (* | fold_matchdecl _ _ _ => fail 1
+   *)| _ => 
+    idtac "evaluating" l;
+    let l' := eval lazy in l in
+    let C' := context C [ fold_matchdecl l' p g] in
+    convert_concl_no_check C'
+  end
+end.
+
+Ltac show_match :=
+  match goal with
+  |- context [match ?x with _ => _ end] => 
+    match x with
+    | match _ with _ => _ end => fail 1
+    | fold_matchdecl _ _ _ => fail 1
+    | _ => idtac x
+    end
+  end.
+
+
+Goal exists  r, test plusr = r.
+Proof.
+  eexists.
+  unfold  test.
+  unfold erase_and_print_template_program.
+  unfold erase_template_program.
+  unfold bind.
+  unfold PCUICSafeChecker.envcheck_monad.
+  fold_matchdecls'.
+  eval_first.
+  show_match.
+
+*)
